add Type-Level Translation

codes/TPTS.v
@@ -1,3 +1,10 @@
+From Stdlib Require Import List.
+From Stdlib Require Import Classical.
+From Stdlib Require Import Logic.IndefiniteDescription.
+Import ListNotations.
+From Stdlib.Program Require Import Program Wf.
+From Stdlib Require Import Lia.
+Require Import Stdlib.Arith.Arith.
 Require Import Thesis.TPTSSignature.
 Require Import Thesis.PTS.
 
@@ -5,5 +12,302 @@ Module TPTS (Sig : TPTS_SIGNATURE).
 Import Sig.
 Module Base := PTS Sig.
 Import Base.
+
+Fixpoint deg (t : term) : nat :=
+  match t with
+  | t_sort s    => index_of s + 1
+  | t_var x     => index_of (var_sort x) - 1
+  | t_pi _ _ B  => deg B
+  | t_lam _ _ M => deg M
+  | t_app M _   => deg M
+  end.
+
+Definition T_eq (j : nat) (M : term) : Prop := deg M = j.
+Definition T_geq (j : nat) (M : term) : Prop := j <= deg M.
+
+Notation "'T_[' j ]" := (T_eq j) (at level 0).
+Notation "'T_≥[' j ]" := (T_geq j) (at level 0).
+
+Definition derivable (M : term) : Prop := exists Γ N, Γ ⊢ M ∈ N.
+
+Lemma deg_typing_succ : forall Γ M N, Γ ⊢ M ∈ N -> deg N = deg M + 1.
+Proof.
+  intros Γ M N Htyp. induction Htyp; simpl in *.
+
+  - apply A_spec in H as [H1 H2]. lia.
+
+  - pose proof (index_range (var_sort x)) as [H1 H2]. lia.
+
+  - exact IHHtyp1.
+
+  - assert (Hshape : s = s') by (apply (R_shape (var_sort x) s s'); exact H).
+    subst s'. exact IHHtyp2.
+
+  - exact IHHtyp1.
+
+  - (* typing_app *)
+    admit.
+
+  - (* typing_conv : M unchanged, type changes A -> B via =b *)
+    admit.
+Admitted.
+
+Lemma deg_le_top : forall M, deg M <= n + 1.
+Proof.
+  induction M; simpl; auto.
+  - pose proof (index_range s) as [_ H]. lia.
+  - pose proof (index_range (var_sort v)) as [_ H]. lia.
+Qed.
+
+Lemma deg_top : forall M, (derivable M) ->
+  (deg M = n + 1 <-> exists s, M = t_sort s /\ index_of s = n).
+Proof.
+  intros M [Γ [N Htyp]]. split.
+
+  - intros Hdeg. induction Htyp.
+    + exists s. split; [reflexivity |]. simpl in Hdeg. lia.
+    + simpl in Hdeg. pose proof (index_range (var_sort x)) as [H1 H2]. lia.
+    + apply IHHtyp1. exact Hdeg.
+    + exfalso. simpl in Hdeg.
+      assert (Hsucc : deg (t_sort s) = deg B + 1) by (apply deg_typing_succ with (Γ ++ [(x, A0)]); exact Htyp2).
+      simpl in Hsucc. pose proof (index_range s) as [_ Hs2]. lia.
+    + exfalso. simpl in Hdeg.
+      assert (Hsucc1 : deg (t_sort s') = deg (t_pi x A0 B) + 1) by (apply deg_typing_succ with (Γ); exact Htyp2).
+      assert (Hsucc2 : deg (B) = deg (M) + 1) by (apply deg_typing_succ with (Γ ++ [(x, A0)]); exact Htyp1).
+      simpl in *. pose proof (index_range s') as [_ Hs2]. lia.
+    + exfalso. simpl in Hdeg.
+      assert (Hsucc : deg (t_pi x A0 B) = deg M + 1) by (apply deg_typing_succ with Γ; exact Htyp1).
+      simpl in Hsucc. pose proof (deg_le_top B) as HB. lia.
+    + apply IHHtyp1. exact Hdeg.
+  
+  - intros [s [Heq Hidx]]. subst M. simpl. lia.
+Qed.
+
+Lemma deg_top_type : forall M, (derivable M) ->
+  deg M = n <-> exists Γ s, (Γ ⊢ M ∈ t_sort s /\ index_of s = n).
+Proof.
+  intros M [Γ [N Htyp]]. split.
+
+  - intros Hdeg. induction Htyp.
+
+    + exists [], s'. split.
+      * apply typing_axiom. exact H.
+      * pose proof (A_spec s s') as [HA _]. apply HA in H as [_ H]. simpl in *. lia.
+
+    + pose proof ((deg_typing_succ Γ A0 (t_sort (var_sort x))) Htyp).
+      simpl in *. assert (HA0 : index_of (var_sort x) = deg A0) by lia.
+      pose proof (index_range (var_sort x)). lia.
+
+    + apply IHHtyp1. apply Hdeg.
+
+    + pose proof ((deg_typing_succ (Γ ++ [(x, A0)]) B (t_sort s)) Htyp2).
+      simpl in *. assert (Hs : index_of s = n) by lia.
+      apply IHHtyp2 in Hdeg. pose proof (R_shape (var_sort x) s s' H) as Heq.
+      subst. exists Γ, s'. split; auto. apply typing_pi with s'; auto.
+
+    + pose proof ((deg_typing_succ (Γ ++ [(x, A0)]) M B) Htyp1).
+      pose proof ((deg_typing_succ Γ (t_pi x A0 B) (t_sort s')) Htyp2).
+      simpl in *. assert (Hs : index_of s' = n + 1) by lia.
+      pose proof (index_range (s')). lia.
+
+    + simpl in Hdeg.
+      pose proof (deg_typing_succ Γ M (t_pi x A0 B) Htyp1) as Hsucc1.
+      simpl in Hsucc1.
+      assert (HdegB : deg B = n + 1) by lia.
+      assert (Hderiv_pi : exists s', Γ ⊢ t_pi x A0 B ∈ t_sort s').
+      { destruct (type_correctness Γ M (t_pi x A0 B) Htyp1) as [[s Hcontra] | [s' Hs']].
+        - discriminate Hcontra.
+        - exists s'. exact Hs'. }
+      destruct Hderiv_pi as [s' Hs'].
+      pose proof (generation_pi Γ x A0 B (t_sort s') Hs')
+        as [sB [sB' [HA0typ [HBtyp [HR Heqs]]]]].
+      assert (Hderiv_B : derivable B) by (exists (Γ ++ [(x, A0)]), (t_sort sB); exact HBtyp).
+      apply (proj1 (deg_top B Hderiv_B)) in HdegB as [s0 [HBeq Hidx0]].
+      subst B.
+      pose proof (deg_typing_succ (Γ ++ [(x, A0)]) (t_sort s0) (t_sort sB) HBtyp) as Hsucc2.
+      simpl in Hsucc2.
+      rewrite Hidx0 in Hsucc2.
+      pose proof (index_range sB) as [_ HsBrange].
+      lia.
+
+    + apply IHHtyp1. exact Hdeg.
+
+  - intros [Γ' [s [H1 H2]]].
+    pose proof (deg_typing_succ Γ' M (t_sort s) H1). simpl in H. lia.
+Qed.
+
+Lemma deg_typing : forall M, derivable M -> forall i, (i > 0) -> (i < n) ->
+  (deg M = i <-> (exists Γ N s, (Γ ⊢ M ∈ N) /\ (Γ ⊢ N ∈ t_sort s) /\ (index_of s = i + 1))).
+Proof.
+  intros M [Γ [T Htyp]] i Hi1 Hi2. split.
+
+  - intros Hdeg. pose proof (deg_typing_succ Γ M T Htyp).
+    pose proof (type_correctness Γ M T Htyp) as Hcor. destruct Hcor as [[s Hs] | [s Hs]].
+    + subst T. simpl in *. pose proof (index_range s). assert (G : index_of s = i) by lia.
+      assert (Hi : 0 < i + 1 < n + 1) by lia.
+      pose proof (index_surj (i + 1) Hi) as Hs'. destruct Hs' as [s' Hs'].
+      assert (Hss' : A s s') by (apply A_spec; lia).
+      exists Γ, (t_sort s), s'. repeat split; auto. apply start_axiom; auto.
+      exists M, (t_sort s); auto.
+    + pose proof (deg_typing_succ Γ T (t_sort s) Hs). simpl in *.
+      exists Γ, T, s. repeat split; auto; lia.
+
+  - intros [Γ' [N [s [H1 [H2 H3]]]]].
+    pose proof (deg_typing_succ Γ' M N H1) as Hdeg1.
+    pose proof (deg_typing_succ Γ' N (t_sort s) H2) as Hdeg2.
+    simpl in *. lia.
+Qed.
+
+Lemma deg_rename : forall M x y, var_sort x = var_sort y -> deg (rename x y M) = deg M.
+Proof.
+  intros M x y Hs. induction M; auto.
+  - simpl. destruct (eq_var_dec v x); auto. subst. simpl. rewrite Hs; auto.
+  - simpl. destruct (eq_var_dec v x); auto.
+  - simpl. destruct (eq_var_dec v x); auto.
+Qed.
+
+Lemma deg_subst : forall M N x j, 
+  (index_of (var_sort x) = j) ->
+  (deg N = j - 1) ->
+  (deg(M⁅x ≔ N⁆) = deg M).
+Proof.
+  intros M N x j Hx Hdeg. induction M.
+  - rewrite subst_sort; auto.
+  - rewrite subst_var. destruct (eq_var_dec v x); auto. subst; auto.
+  - rewrite subst_app; auto.
+  - rewrite subst_lam. simpl. 
+    remember (fresh (var_sort v) (fv N ++ fv M2)) as z.
+    remember (rename v z M2) as M2r.
+    assert (Hs : var_sort v = var_sort z). rewrite Heqz; auto.
+    pose proof (deg_rename M2 v z Hs).
+    rewrite <- HeqM2r in *. admit.
+  - rewrite subst_pi. simpl.
+    remember (fresh (var_sort v) (fv N ++ fv M2)) as z.
+    remember (rename v z M2) as M2r.
+    assert (Hs : var_sort v = var_sort z). rewrite Heqz; auto.
+    pose proof (deg_rename M2 v z Hs).
+    rewrite <- HeqM2r in *. admit.
+Admitted.
+
+Lemma deg_beta : forall M N, (M ->>b N) -> (deg M = deg N).
+Proof.
+  intros M B Hbeta. induction Hbeta; auto.
+  - induction H; auto. simpl. symmetry. 
+    apply deg_subst with (index_of (var_sort x)); auto.
+    admit.
+  - rewrite IHHbeta1. rewrite <- IHHbeta2. reflexivity.
+Admitted.
+
+Definition full_with (i j : nat) : Prop :=
+  forall l k : Sort,
+  index_of l <= i ->
+  index_of l <= index_of k ->
+  index_of k <= j ->
+  R l k k.
+
+Definition full : Prop :=
+  forall s1 s2 s3, R s1 s2 s3 -> full_with (index_of s2) (index_of s1).
+
+(* For the remainder of this section, fix a full n-tiered pure type system λS. *)
+Axiom is_full : full.
+
+Definition R_star (s s' s'' : Sort) : Prop :=
+  R s s' s'' /\ index_of s' <= index_of s.
+
+Reserved Notation "Γ ⊢* M ∈ A" (at level 70, no associativity).
+
+Inductive typing_star : context -> term -> term -> Prop :=
+  | typing_star_axiom : forall s s',
+      A s s' ->
+      [] ⊢* t_sort s ∈ t_sort s'
+
+  | typing_star_var : forall Γ x A,
+      is_fresh x Γ ->
+      Γ ⊢* A ∈ t_sort (var_sort x) ->
+      Γ ++ [(x, A)] ⊢* t_var x ∈ A
+
+  | typing_star_weak : forall Γ x B M A,
+      is_fresh x Γ ->
+      Γ ⊢* M ∈ A ->
+      Γ ⊢* B ∈ t_sort (var_sort x) ->
+      Γ ++ [(x, B)] ⊢* M ∈ A
+
+  | typing_star_pi : forall Γ x A B s s',
+      Γ ⊢* A ∈ t_sort (var_sort x) ->
+      Γ ++ [(x, A)] ⊢* B ∈ t_sort s ->
+      R_star (var_sort x) s s' ->
+      Γ ⊢* (t_pi x A B) ∈ (t_sort s')
+
+  | typing_star_lam : forall Γ x A M B s',
+      Γ ++ [(x, A)] ⊢* M ∈ B ->
+      Γ ⊢* (t_pi x A B) ∈ (t_sort s') ->
+      Γ ⊢* (t_lam x A M) ∈ (t_pi x A B)
+
+  | typing_star_app : forall Γ M N A B x,
+      Γ ⊢* M ∈ t_pi x A B ->
+      Γ ⊢* N ∈ A ->
+      Γ ⊢* t_app M N ∈ (B⁅x ≔ N⁆)
+
+  | typing_star_conv : forall Γ M A B s,
+      Γ ⊢* M ∈ A ->
+      A =b B ->
+      Γ ⊢* B ∈ t_sort s ->
+      Γ ⊢* M ∈ B
+
+where "Γ ⊢* M ∈ A" := (typing_star Γ M A).
+
+Definition legal_star (Γ : context) : Prop :=
+  exists M N, Γ ⊢* M ∈ N.
+
+Definition derivable_star (M : term) : Prop :=
+  exists Γ N, Γ ⊢* M ∈ N.
+
+Definition partial_sort_of (i : nat) (Hi : 0 < i < n + 1) : Sort :=
+  proj1_sig (
+    constructive_indefinite_description
+      (fun s => index_of s = i)
+      (index_surj i Hi)
+  ).
+
+Lemma one_in_range : 0 < 1 /\ 1 < n + 1.
+Proof. pose proof n_range. lia. Qed.
+
+Definition sort_of (i : nat) : Sort :=
+  match (lt_dec 0 i, lt_dec i (n+1)) with
+  | (left H1, left H2) => partial_sort_of i (conj H1 H2)
+  | _ => partial_sort_of 1 one_in_range
+  end.
+
+(* Type-Level Translation *)
+Parameter zero_var : var.
+
+Fixpoint rho (i : nat) (M : term) : term :=
+  match M with
+  | t_sort s =>
+      match i with
+      | 0 => t_var zero_var
+      | _ => t_sort (sort_of i)
+      end
+  | t_var x =>
+      t_var (mkvar (sort_of (i + 2)) (var_idx x))
+  | t_pi x A B =>
+      (fix pi_tel (k : nat) : term :=
+         match k with
+         | 0    => t_pi x (rho i A) (rho i B)
+         | S k' => t_pi x (rho (i + S k') A) (pi_tel k')
+         end) (deg A - 1 - i)
+  | t_lam x A M' =>
+      (fix lam_tel (k : nat) : term :=
+         match k with
+         | 0    => t_lam x (rho (i + 1) A) (rho i M')
+         | S k' => t_lam x (rho (i + 1 + S k') A) (lam_tel k')
+         end) (deg A - 1 - (i + 1))
+  | t_app M' N =>
+      (fix app_tel (k : nat) : term :=
+         match k with
+         | 0    => t_app (rho i M') (rho i N)
+         | S k' => t_app (app_tel k') (rho (i + S k') N)
+         end) (deg N - 1 - i)
+  end.
 
 End TPTS.
